start implementing new word translation

src/HOL/Library/Word.thy
@@ -4751,26 +4751,17 @@ lemma slice_lift:
 (*
 Lifting from operators that should be natively translated into SMT-LIB that take in natural numbers
 or return them to operators that work only on integers.
-
-TODO: These are not about natural numbers anymore so we should change the name or make another
-set. They should always
-be done no matter if smt_nat_as_int is activated
 *)
 
 
-definition push_bit_lift :: \<open>'a::len word  \<Rightarrow> 'a::len word \<Rightarrow> 'a::len word\<close> where
-  "push_bit_lift w k = push_bit (unat k) w"
+definition push_bit_lift :: \<open>'a::len word  \<Rightarrow> int \<Rightarrow> 'a::len word\<close> where
+  "push_bit_lift w k = (if k > LENGTH('a) \<or> k < 0 then 0 else push_bit (nat k) w)"
 
 lemma push_bit_lift:
- "push_bit k (w::'a::len word) \<equiv> (if k > LENGTH('a) then 0 else push_bit_lift w (Word.Word k))"
+ "push_bit k (w::'a::len word) \<equiv> push_bit_lift w k"
   unfolding push_bit_lift_def
-  apply (simp add: atomize_eq)
-  apply (cases "k > LENGTH('a)")
-   apply simp_all
-  apply (simp add: unsigned_of_nat take_bit_nat_eq_self_iff)
-  by (metis dual_order.strict_trans less_exp nat_neq_iff take_bit_nat_eq_self_iff)
-
-
+  by (simp add: atomize_eq)
+  
 definition drop_bit_lift :: \<open>'a::len word  \<Rightarrow> 'a::len word \<Rightarrow> 'a::len word\<close> where
   "drop_bit_lift w k = drop_bit (unat k) w"
 
@@ -4870,20 +4861,6 @@ lemma [nat_normalized_input]:
   "smt_extract (nat j) (nat i) w \<equiv> smt_extract_lift j i w"
   unfolding smt_extract_lift_def by simp
 
-definition bit_lift :: \<open>'a::len word \<Rightarrow> int \<Rightarrow> bool\<close> where
-  "bit_lift w x = bit w (nat x)"
-lemma bit_lift:
-  "bit w x \<equiv> bit_lift w (int x)"
-  unfolding bit_lift_def by simp
-(*
-We want to translate to smt_extract if the condition is met... Do we want to normalize here already?
- "k < size (x::'a::len word) \<Longrightarrow> bit x k = ((smt_extract k k x) = (1::1 word))"
-*)
-  
-lemma [nat_normalized_input]:
-  "bit w (nat x) \<equiv> bit_lift w x"
-  unfolding bit_lift_def by simp
-
 
 lemma [nat_normalized_input]:
   "ucast w \<equiv> Word.cast w"
@@ -4908,7 +4885,6 @@ val nat_native_ops_tab =
   ("Bit_Operations.semiring_bit_operations_class.take_bit",@{thms take_bit_lift}),
   ("Bit_Operations.semiring_bit_operations_class.drop_bit",@{thms drop_bit_lift}),
   ("Bit_Operations.semiring_bit_operations_class.push_bit", @{thms push_bit_lift}),
-  ("Bit_Operations.semiring_bits_class.bit", @{thms bit_lift}),
   ("Word.word_rotr", @{thms word_rotr_lift}),
   ("Word.word_rotl", @{thms word_rotl_lift}),
   ("Word.smt_extract", @{thms smt_extract_lift})
@@ -4946,5 +4922,9 @@ val _ = fold SMT_Normalize.add_simplify_ops_tab (simplify_norm_table)
 
 declare [[smt_nat_as_int]]
 lemmas [smt_word_len_evaluate] = semiring_numeral_class.numeral_times_numeral
+
+lemma "push_bit (4::nat) (3::8 word) \<noteq> 0"
+  supply[[smt_trace]]
+  apply (smt (cvc5))
 
 end
